src/Lustre/Normalization/NTyping.v
@@ -62,6 +62,18 @@ Module Type NTYPING
     rewrite typesof_annots, H, <- typeof_annot...
   Qed.
 
+  Corollary map_bind2_normalize_exp_typesof'' : forall G vars is_control es es' eqs' st st',
+      Forall (wt_exp G vars) es ->
+      map_bind2 (normalize_exp is_control) es st = (es', eqs', st') ->
+      Forall2 (fun e ty => typeof e = [ty]) (concat es') (typesof es).
+  Proof.
+    intros * Hwl Hmap.
+    eapply map_bind2_normalize_exp_annots'' in Hmap; eauto.
+    rewrite typesof_annots, Forall2_map_2.
+    eapply Forall2_impl_In; eauto. intros; simpl in *.
+    rewrite typeof_annot, H1; auto.
+  Qed.
+
   Corollary map_bind2_normalize_exp_typesof :
     forall G vars is_control es es' eqs' st st',
       Forall (wt_exp G vars) es ->
@@ -216,24 +228,28 @@ Module Type NTYPING
 
   Fact idents_for_anns_wt : forall G vars anns ids st st',
       idents_for_anns anns st = (ids, st') ->
-      Forall (fun '(ty, cl) => wt_nclock vars cl) anns ->
-      Forall (wt_exp G (vars++(idty ids))) (map (fun '(x, ann) => Evar x ann) ids).
+      Forall (fun '(ty, cl) => wt_nclock (vars++st_tys st) cl) anns ->
+      Forall (wt_exp G (vars++st_tys st')) (map (fun '(x, ann) => Evar x ann) ids).
   Proof.
     induction anns; intros ids st st' Hidents Hf;
       repeat inv_bind.
     - constructor.
     - inv Hf. destruct a as [ty [cl ?]]. repeat inv_bind.
+      assert (Forall (fun '(_, cl) => wt_nclock (vars ++ st_tys x0) cl) anns) as Hanns'.
+      { solve_forall. repeat solve_incl. }
       rewrite Forall_map.
-      specialize (IHanns x1 _ _ H0 H2).
-      econstructor; eauto.
+      eapply IHanns in Hanns'; eauto.
+      econstructor.
       + repeat constructor; simpl.
-        * apply in_or_app. right. constructor; auto.
+        * apply in_or_app; right.
+          apply fresh_ident_In in H.
+          rewrite st_anns_tys_In. exists cl. exists false.
+          eapply idents_for_anns_st_follows, st_follows_incl in H0; eauto.
         * inv H1. repeat solve_incl.
-      + rewrite Forall_map in IHanns.
-        solve_forall. repeat solve_incl.
+      + simpl_forall.
   Qed.
 
-  Fact idents_for_anns'_wt_exp : forall G vars anns ids st st',
+  Fact idents_for_anns'_wt : forall G vars anns ids st st',
       idents_for_anns' anns st = (ids, st') ->
       Forall (fun '(ty, cl) => wt_nclock (vars++(idty ids)++st_tys st) cl) anns ->
       Forall (wt_exp G (vars++(idty ids)++st_tys st')) (map (fun '(x, ann) => Evar x ann) ids).
@@ -248,12 +264,12 @@ Module Type NTYPING
         * apply in_or_app. right. constructor; auto.
         * inv H1. destruct x; simpl in *. solve_incl.
           eapply incl_appr', incl_tl', incl_appr'. solve_incl.
-      + eapply IHanns in H0.
+      + destruct x. eapply IHanns in H0.
         * rewrite Forall_map in H0.
           solve_forall. repeat solve_incl.
-        * solve_forall. destruct a, x. solve_incl.
+        * solve_forall. solve_incl.
           rewrite Permutation.Permutation_middle.
-          eapply incl_appr', incl_appr', incl_cons; try solve_incl.
+          eapply incl_appr', incl_appr', incl_cons; repeat solve_incl.
           eapply reuse_ident_In in H. unfold st_tys, idty, idty.
           rewrite in_map_iff. exists (i, (ty, cl)); split; auto.
           rewrite in_map_iff. eexists; split; [|eauto]; eauto.
@@ -264,7 +280,7 @@ Module Type NTYPING
       + eapply IHanns in H0.
         * rewrite Forall_map in H0.
           solve_forall. repeat solve_incl.
-        * solve_forall. destruct a. solve_incl.
+        * solve_forall. solve_incl.
           rewrite Permutation.Permutation_middle.
           eapply incl_appr', incl_appr', incl_cons; try solve_incl.
           eapply fresh_ident_In in H. unfold st_tys, idty, idty.
@@ -354,357 +370,271 @@ Module Type NTYPING
         * etransitivity; eauto.
   Qed.
 
-  Fact normalize_exp_wt_exp : forall G vars e is_control es' eqs' st st',
+  Fact normalize_when_wt_exp : forall G vars b ckid es tys ck,
+      In (ckid, Op.bool_type) vars ->
+      wt_nclock vars ck ->
+      Forall (wt_exp G vars) es ->
+      Forall2 (fun e ty => typeof e = [ty]) es tys ->
+      Forall (wt_exp G vars) (normalize_when ckid b es tys ck).
+  Proof.
+    intros * HIn Hwtck Hwt Htys. unfold normalize_when.
+    assert (length es = length tys) as Hlength by (eapply Forall2_length in Htys; eauto).
+    rewrite Forall_map. apply Forall2_combine'.
+    eapply Forall2_ignore2' with (ys:=tys) in Hwt; eauto.
+    eapply Forall2_Forall2 in Hwt; eauto. clear Htys.
+    eapply Forall2_impl_In; eauto. intros ? ? ? ? [? ?].
+    repeat constructor; simpl; auto.
+    rewrite app_nil_r; auto.
+  Qed.
+
+  Fact normalize_merge_wt_exp : forall G vars ckid ets efs tys ck,
+      In (ckid, Op.bool_type) vars ->
+      wt_nclock vars ck ->
+      Forall (wt_exp G vars) ets ->
+      Forall (wt_exp G vars) efs ->
+      Forall2 (fun e ty => typeof e = [ty]) ets tys ->
+      Forall2 (fun e ty => typeof e = [ty]) efs tys ->
+      Forall (wt_exp G vars) (normalize_merge ckid ets efs tys ck).
+  Proof with eauto.
+    intros * HIn Hwtck Hwt1 Hwt2 Htys1 Htys2. unfold normalize_merge.
+    assert (length ets = length tys) as Hlen1 by (eauto using Forall2_length).
+    assert (length efs = length tys) as Hlen2 by (eauto using Forall2_length).
+    solve_forall.
+    repeat constructor; simpl; auto. 1,2:rewrite app_nil_r; auto.
+  Qed.
+
+  Fact normalize_ite_wt_exp : forall G vars e ets efs tys ck,
+      wt_nclock vars ck ->
       wt_exp G vars e ->
+      typeof e = [Op.bool_type] ->
+      Forall (wt_exp G vars) ets ->
+      Forall (wt_exp G vars) efs ->
+      Forall2 (fun e ty => typeof e = [ty]) ets tys ->
+      Forall2 (fun e ty => typeof e = [ty]) efs tys ->
+      Forall (wt_exp G vars) (normalize_ite e ets efs tys ck).
+  Proof with eauto.
+    intros * Hwtck Hwt Htye Hwt1 Hwt2 Htys1 Htys2. unfold normalize_ite.
+    assert (length ets = length tys) as Hlen1 by (eauto using Forall2_length).
+    assert (length efs = length tys) as Hlen2 by (eauto using Forall2_length).
+    solve_forall.
+    repeat constructor; simpl; auto. 1,2:rewrite app_nil_r; auto.
+  Qed.
+
+  Lemma normalize_exp_wt_exp : forall G vars e is_control es' eqs' st st',
+      wt_exp G (vars++st_tys st) e ->
       normalize_exp is_control e st = (es', eqs', st') ->
       Forall (wt_exp G (vars++st_tys st')) es'.
   Proof with eauto.
-    intros G vars e is_control es' eqs' st st' Hwt;
-      revert is_control eqs' es' st st'.
-    induction Hwt using wt_exp_ind2;
-      intros is_control eqs' es' st st' Hnorm; simpl in *.
+    induction e using exp_ind2; intros * Hwt Hnorm; inv Hwt; simpl in *.
     - (* const *)
       repeat inv_bind...
     - (* var *)
       repeat inv_bind.
-      repeat constructor.
-      + apply in_or_app...
-      + repeat solve_incl.
+      repeat constructor...
     - (* unop *)
       repeat inv_bind.
-      specialize (IHHwt _ _ _ _ _ H2).
-      repeat constructor.
       assert (length x = numstreams e) as Hlen by eauto.
-      rewrite <- length_typeof_numstreams in Hlen.
-      replace (typeof e) in *.
+      rewrite <- length_typeof_numstreams, H3 in Hlen; simpl in Hlen.
       singleton_length.
-      inv IHHwt. econstructor...
-      eapply normalize_exp_typeof in Hwt...
-      simpl in *; rewrite app_nil_r in Hwt; rewrite Hwt...
-      eapply wt_nclock_incl; [| eauto]...
+      assert (Hnorm:=H); eapply IHe in H; eauto.
+      repeat econstructor...
+      + inv H; eauto.
+      + eapply normalize_exp_typeof in Hnorm; simpl in Hnorm; eauto.
+        rewrite app_nil_r, H3 in Hnorm...
+      + repeat solve_incl.
     - (* binop *)
       repeat inv_bind.
-      specialize (IHHwt1 _ _ _ _ _ H3).
-      specialize (IHHwt2 _ _ _ _ _ H4).
-      repeat constructor.
       assert (length x = numstreams e1) as Hlen1 by eauto.
+      rewrite <- length_typeof_numstreams, H5 in Hlen1; simpl in Hlen1.
       assert (length x2 = numstreams e2) as Hlen2 by eauto.
-      rewrite <- length_typeof_numstreams in Hlen1.
-      rewrite <- length_typeof_numstreams in Hlen2.
-      replace (typeof e1) in *.
-      replace (typeof e2) in *.
-      repeat singleton_length.
-      eapply normalize_exp_typeof in Hwt1...
-      eapply normalize_exp_typeof in Hwt2...
-      inv IHHwt1. inv IHHwt2.
-      econstructor; eauto;
-        simpl in *; rewrite app_nil_r in *;
-          try rewrite Hwt1; try rewrite Hwt2...
-      + eapply normalize_exp_st_follows in H3. repeat solve_incl.
+      rewrite <- length_typeof_numstreams, H6 in Hlen2; simpl in Hlen2. repeat singleton_length.
+      assert (Hnorm1:=H); eapply IHe1 in H; eauto.
+      assert (Hnorm2:=H0); eapply IHe2 in H0; eauto. 2:repeat solve_incl.
+      repeat econstructor...
+      + inv H. repeat solve_incl.
+      + inv H0...
+      + eapply normalize_exp_typeof in Hnorm1; simpl in Hnorm1; eauto.
+        rewrite app_nil_r, H5 in Hnorm1...
+      + eapply normalize_exp_typeof in Hnorm2; simpl in Hnorm2; eauto.
+        rewrite app_nil_r, H6 in Hnorm2...
       + repeat solve_incl.
     - (* fby *)
       repeat inv_bind.
-      specialize (idents_for_anns_incl_ty _ _ _ _ H9) as Hincl.
-      apply idents_for_anns_wt with (G:=G) (vars:=vars) in H9.
-      + solve_forall.
-        eapply wt_exp_incl; [| eauto].
-        apply incl_app...
-      + rewrite Forall_forall in *; intros.
-        destruct x as [? [? ?]]. eapply H5.
-        simpl_In.
-        exists (t, (c, o)); simpl...
+      eapply idents_for_anns_wt in H9...
+      rewrite Forall_map in H8.
+      solve_forall. repeat solve_incl.
     - (* when *)
       repeat inv_bind.
-      assert (length (concat x1) = length (annots es)) as Hlength by eauto.
-      assert (typesof (concat x1) = typesof es) as Htypeof by eauto.
-      repeat rewrite_Forall_forall.
-      rewrite in_map_iff in H4; destruct H4 as [[? ?] [? Hin]]; subst.
-      constructor; simpl.
-      + repeat constructor. eapply map_bind2_wt_exp in H1.
-        * rewrite Forall_forall in H1...
-        * intros; eapply normalize_exp_st_follows...
-        * rewrite Forall_forall; intros.
-          eapply H0 in H5; eauto.
-          solve_forall. repeat solve_incl.
-      + rewrite app_nil_r.
-        specialize (map_bind2_normalize_exp_numstreams _ _ _ _ _ _ H1) as Hnumstreams.
-        eapply map_bind2_normalize_exp_typesof in H1; [| rewrite Forall_forall; intros; auto].
-        rewrite <- Htypeof in Hin.
-        repeat simpl_nth.
-        repeat simpl_list.
-        eapply concat_length_map_nth; solve_forall.
-        * repeat solve_length.
-        * rewrite length_typeof_numstreams...
-      + apply in_or_app...
+      eapply normalize_when_wt_exp; eauto.
+      + assert (incl (vars ++ st_tys st) (vars ++ st_tys st')) as Hincl by repeat solve_incl...
       + repeat solve_incl.
+      + eapply map_bind2_wt_exp in H0; eauto.
+        solve_forall. eapply H5 in H2...
+        solve_forall. 1,2:repeat solve_incl.
+      + eapply map_bind2_normalize_exp_typesof'' in H0; eauto.
     - (* merge *)
+      repeat inv_bind.
+      assert (Forall (wt_exp G (vars ++ st_tys x2)) (concat x3)) as Hwt1.
+      { eapply map_bind2_wt_exp in H1; eauto.
+        eapply Forall_Forall in H; eauto.
+        eapply Forall_impl; eauto.
+        intros ? [? ?] ? ? ? ? ? ? ?. eapply H8 in H11; eauto.
+        solve_forall; eauto. 1,2:repeat solve_incl. }
+      assert (Forall (wt_exp G (vars ++ st_tys x5)) (concat x6)) as Hwt2.
+      { eapply map_bind2_wt_exp in H2; eauto.
+        solve_forall. eapply H11 in H5...
+        solve_forall. 1,2:repeat solve_incl. } clear H H0.
       destruct is_control; repeat inv_bind.
-      + rewrite Forall_map.
-        rewrite Forall_forall; intros [[et ef] ty] Hin.
-        assert (length (concat x3) = length (annots ets)) by eauto.
-        assert (length (concat x5) = length (annots efs)) by eauto.
-        constructor; simpl.
-        * eapply map_bind2_wt_exp with (G0:=G) (vars0 := (vars++(st_tys x2))) in H7...
-          -- repeat constructor.
-             repeat simpl_In.
-             rewrite Forall_forall in H7. apply H7 in H11.
-             repeat solve_incl.
-          -- clear H1 H2.
-             repeat rewrite_Forall_forall. apply H0 in H2...
-             rewrite_Forall_forall. apply H2 in H12. repeat solve_incl.
-        * eapply map_bind2_wt_exp with (G0:=G) (vars0 := (vars++(st_tys st'))) in H4...
-          -- repeat constructor.
-             repeat simpl_In.
-             rewrite Forall_forall in H4. apply H4 in H10.
-             repeat solve_incl.
-          -- clear H H0.
-             repeat rewrite_Forall_forall. eapply H2 in H0...
-             rewrite_Forall_forall. apply H0 in H12. repeat solve_incl.
-        * apply in_or_app...
-        * rewrite app_nil_r.
-          specialize (map_bind2_normalize_exp_numstreams _ _ _ _ _ _ H7) as Hnumstreams.
-          eapply map_bind2_normalize_exp_typesof in H7; [| rewrite Forall_forall in *; intros; auto].
-          rewrite <- H7 in Hin. rewrite <- length_typesof_annots in *.
-          repeat simpl_nth.
-          repeat simpl_list.
-          eapply concat_length_map_nth; solve_forall.
-          -- repeat solve_length.
-          -- rewrite length_typeof_numstreams...
-        * rewrite app_nil_r.
-          specialize (map_bind2_normalize_exp_numstreams _ _ _ _ _ _ H4) as Hnumstreams.
-          eapply map_bind2_normalize_exp_typesof in H4; [| rewrite Forall_forall in *; intros; auto].
-          rewrite <- H5 in Hin. rewrite <- H4 in Hin. rewrite <- length_typesof_annots in *.
-          repeat simpl_nth.
-          repeat simpl_list.
-          eapply concat_length_map_nth; solve_forall.
-          -- repeat solve_length.
-          -- rewrite length_typeof_numstreams...
+      + eapply normalize_merge_wt_exp; auto.
+        * assert (incl (vars ++ st_tys st) (vars ++ st_tys st')) as Hincl by repeat solve_incl...
         * repeat solve_incl.
-      + specialize (idents_for_anns_incl_ty _ _ _ _ H9) as Hincl.
-        apply idents_for_anns_wt with (G:=G) (vars:=vars) in H9.
-        * solve_forall. repeat solve_incl...
-        * rewrite Forall_forall; intros.
-          repeat simpl_In. inv H8...
-    - (* ite *)
-      destruct is_control; repeat inv_bind.
-      + rewrite Forall_map.
-        rewrite Forall_forall; intros [[et ef] ty] Hin.
-        assert (length (concat x5) = length (annots ets)) by eauto.
-        assert (length (concat x7) = length (annots efs)) by eauto.
-        constructor; simpl...
-        * apply IHHwt in H7...
-          apply hd_default_wt_exp. solve_forall.
-          apply map_bind2_st_follows in H8; solve_forall.
-          apply map_bind2_st_follows in H4; solve_forall.
-          repeat solve_incl.
-        * eapply map_bind2_wt_exp with (G0:=G) (vars0 := (vars++(st_tys x4))) in H8...
-          -- repeat constructor.
-             repeat simpl_In.
-             rewrite Forall_forall in H8. apply H8 in H12.
-             repeat solve_incl.
-          -- clear H1 H2 IHHwt.
-             repeat rewrite_Forall_forall. apply H0 in H2...
-             rewrite_Forall_forall. eapply H2 in H13. repeat solve_incl.
-        * eapply map_bind2_wt_exp with (G0:=G) (vars0 := (vars++(st_tys st'))) in H4...
-          -- repeat constructor.
-             repeat simpl_In.
-             rewrite Forall_forall in H4. apply H4 in H11.
-             repeat solve_incl.
-          -- clear H H0 IHHwt.
-             repeat rewrite_Forall_forall. apply H2 in H0...
-             rewrite_Forall_forall. apply H0 in H13. repeat solve_incl.
-        * assert (length x = numstreams e) as Hlength by eauto.
-          rewrite <- length_typeof_numstreams in Hlength.
-          rewrite H3 in Hlength; simpl in Hlength.
-          eapply normalize_exp_typeof in H7...
-          singleton_length. congruence.
-        * rewrite app_nil_r.
-          specialize (map_bind2_normalize_exp_numstreams _ _ _ _ _ _ H8) as Hnumstreams.
-          eapply map_bind2_normalize_exp_typesof in H8; [| rewrite Forall_forall in *; intros; auto].
-          rewrite <- H8 in Hin. rewrite <- length_typesof_annots in *.
-          repeat simpl_nth.
-          repeat simpl_list.
-          eapply concat_length_map_nth; solve_forall.
-          -- repeat solve_length.
-          -- rewrite length_typeof_numstreams...
-        * rewrite app_nil_r.
-          specialize (map_bind2_normalize_exp_numstreams _ _ _ _ _ _ H4) as Hnumstreams.
-          eapply map_bind2_normalize_exp_typesof in H4; [| rewrite Forall_forall in *; intros; auto].
-          rewrite <- H5 in Hin. rewrite <- H4 in Hin. rewrite <- length_typesof_annots in *.
-          repeat simpl_nth.
-          repeat simpl_list.
-          eapply concat_length_map_nth; solve_forall.
-          -- repeat solve_length.
-          -- rewrite length_typeof_numstreams...
-        * repeat solve_incl.
-      + specialize (idents_for_anns_incl_ty _ _ _ _ H10) as Hincl.
-        apply idents_for_anns_wt with (G:=G) (vars:=vars) in H10.
         * solve_forall. repeat solve_incl.
-        * rewrite Forall_forall; intros.
-          destruct x2. repeat simpl_In. inv H9...
+        * eapply map_bind2_normalize_exp_typesof'' in H1...
+        * eapply map_bind2_normalize_exp_typesof'' in H2... congruence.
+      + specialize (idents_for_anns_incl_ty _ _ _ _ H) as Hincl.
+        apply idents_for_anns_wt with (G:=G) (vars:=vars) in H...
+        rewrite Forall_forall; intros.
+        repeat simpl_In. inv H0... repeat solve_incl.
+    - (* ite *)
+      repeat inv_bind.
+      assert (length x = 1) as Hlen.
+      { eapply normalize_exp_length in H1...
+        rewrite H1, <- length_typeof_numstreams, H8... } singleton_length.
+      assert (typeof e0 = [Op.bool_type]) as Htyp.
+      { eapply normalize_exp_typeof in H1; simpl in H1...
+        rewrite app_nil_r in H1; congruence. }
+      assert (wt_exp G (vars ++ st_tys x1) e0) as Hwt'.
+      { eapply IHe in H1... inv H1... }
+      assert (Forall (wt_exp G (vars ++ st_tys x4)) (concat x5)) as Hwt1.
+      { eapply map_bind2_wt_exp in H2; eauto.
+        solve_forall. eapply H13 in H7...
+        solve_forall. 1,2:repeat solve_incl. }
+      assert (Forall (wt_exp G (vars ++ st_tys x7)) (concat x8)) as Hwt2.
+      { eapply map_bind2_wt_exp in H3; eauto.
+        solve_forall. eapply H13 in H7...
+        solve_forall. 1,2:repeat solve_incl. } clear H H0.
+      destruct is_control; repeat inv_bind.
+      + eapply normalize_ite_wt_exp; auto.
+        * repeat solve_incl.
+        * repeat solve_incl.
+        * solve_forall. repeat solve_incl.
+        * eapply map_bind2_normalize_exp_typesof'' in H2...
+        * eapply map_bind2_normalize_exp_typesof'' in H3... congruence.
+      + specialize (idents_for_anns_incl_ty _ _ _ _ H) as Hincl.
+        apply idents_for_anns_wt with (G:=G) (vars:=vars) in H...
+        rewrite Forall_forall; intros.
+        repeat simpl_In. inv H0... repeat solve_incl.
     - (* app *)
       repeat inv_bind.
-      specialize (idents_for_anns'_incl_ty _ _ _ _ H6) as Hincl.
-      eapply idents_for_anns'_wt_exp with (G:=G) (vars:=vars) in H6...
+      specialize (idents_for_anns'_incl_ty _ _ _ _ H2) as Hincl.
+      eapply idents_for_anns'_wt with (G:=G) (vars:=vars) in H2...
       + solve_forall. repeat solve_incl.
-      + solve_forall. destruct a; simpl in *...
-        solve_incl. unfold idty. rewrite map_app.
-        eapply incl_appr'. rewrite Permutation.Permutation_app_comm.
-        eapply incl_app; [eapply incl_appl|eapply incl_appr].
-        * apply idents_for_anns'_anon_streams_incl in H6.
-          eapply incl_map in H6. etransitivity. eapply H6.
+      + solve_forall. simpl in *...
+        solve_incl. unfold idty. rewrite map_app, <- app_assoc.
+        apply incl_appr', incl_app; [repeat solve_incl|apply incl_app;[apply incl_appr|apply incl_appl]].
+        * eapply map_bind2_normalize_exp_fresh_incl in H1.
+          unfold st_tys, idty in *. apply incl_map...
+        * eapply idents_for_anns'_anon_streams_incl, incl_map in H2.
+          etransitivity. eapply H2.
           replace (map _ (without_names' x1)) with (map (fun xtc => (fst xtc, fst (snd xtc))) x1); auto.
           unfold without_names'; rewrite map_map; simpl.
           apply map_ext; intros [? [? [? ?]]]; auto.
-        * eapply map_bind2_normalize_exp_fresh_incl in H5.
-          unfold st_tys, idty in *. eapply incl_map; eauto.
     - (* app (reset) *)
       repeat inv_bind.
-      specialize (idents_for_anns'_incl_ty _ _ _ _ H8) as Hincl.
-      eapply idents_for_anns'_wt_exp with (G:=G) (vars:=vars) in H8...
+      specialize (idents_for_anns'_incl_ty _ _ _ _ H3) as Hincl.
+      eapply idents_for_anns'_wt with (G:=G) (vars:=vars) in H3...
       + solve_forall. repeat solve_incl.
-      + solve_forall. destruct a; simpl in *...
-        solve_incl. unfold idty. rewrite map_app.
-        eapply incl_appr'. rewrite Permutation.Permutation_app_comm.
-        eapply incl_app; [eapply incl_appl|eapply incl_appr].
-        * apply idents_for_anns'_anon_streams_incl in H8.
-          eapply incl_map in H8. etransitivity. eapply H8.
-          replace (map _ (without_names' x5)) with (map (fun xtc => (fst xtc, fst (snd xtc))) x5); auto.
-          unfold without_names'; rewrite map_map; simpl.
-          apply map_ext; intros [? [? [? ?]]]; auto.
-        * eapply map_bind2_normalize_exp_fresh_incl in H6.
+      + solve_forall; simpl in *...
+        solve_incl. unfold idty. rewrite map_app, <- app_assoc.
+        apply incl_appr', incl_app; [repeat solve_incl|apply incl_app;[apply incl_appr|apply incl_appl]].
+        * eapply map_bind2_normalize_exp_fresh_incl in H1.
           unfold st_tys, idty in *. eapply incl_map.
           assert (st_follows x1 x4) by repeat solve_st_follows.
           etransitivity... eapply incl_map...
+        * eapply idents_for_anns'_anon_streams_incl, incl_map in H3.
+          etransitivity. eapply H3.
+          replace (map _ (without_names' x5)) with (map (fun xtc => (fst xtc, fst (snd xtc))) x5); auto.
+          unfold without_names'; rewrite map_map; simpl.
+          apply map_ext; intros [? [? [? ?]]]; auto.
   Qed.
 
   Corollary map_bind2_normalize_exp_wt_exp : forall G vars is_control es es' eqs' st st',
-      Forall (wt_exp G vars) es ->
+      Forall (wt_exp G (vars++st_tys st)) es ->
       map_bind2 (normalize_exp is_control) es st = (es', eqs', st') ->
-      Forall (wt_exp G (vars++(st_tys st'))) (concat es').
+      Forall (wt_exp G (vars++st_tys st')) (concat es').
   Proof.
     intros G vars is_control es es' eqs' st st' Hwt Hmap.
     eapply map_bind2_wt_exp in Hmap; solve_forall; eauto.
-    eapply normalize_exp_wt_exp in H0; eauto.
-    solve_forall. repeat solve_incl.
+    eapply normalize_exp_wt_exp with (G:=G) (vars:=vars) in H1; eauto.
+    solve_forall. 1,2:repeat solve_incl.
   Qed.
 
   Corollary normalize_exps_wt_exp : forall G vars es es' eqs' st st',
-      Forall (wt_exp G vars) es ->
+      Forall (wt_exp G (vars++st_tys st)) es ->
       normalize_exps es st = (es', eqs', st') ->
-      Forall (wt_exp G (vars++(st_tys st'))) es'.
+      Forall (wt_exp G (vars++st_tys st')) es'.
   Proof.
     intros G vars es es' eqs' st st' Hwt Hmap.
     unfold normalize_exps in Hmap; repeat inv_bind.
     eapply map_bind2_normalize_exp_wt_exp in H; eauto.
   Qed.
 
-Fact normalize_fby_wt_exp : forall G vars e0s es anns es' eqs' st st',
+  Fact normalize_fby_wt_exp : forall G vars e0s es anns es' eqs' st st',
       Forall (wt_exp G (vars++(st_tys st))) e0s ->
       Forall (wt_exp G (vars++(st_tys st))) es ->
-      Forall2 (fun e0 a => typeof e0 = [fst a]) e0s anns ->
-      Forall2 (fun e a => typeof e = [fst a]) es anns ->
-      Forall (fun '(_, cl) => wt_nclock vars cl) anns ->
+      Forall2 (fun e0 a => typeof e0 = [a]) e0s (map fst anns) ->
+      Forall2 (fun e a => typeof e = [a]) es (map fst anns) ->
+      Forall (fun '(_, cl) => wt_nclock (vars++st_tys st) cl) anns ->
       normalize_fby e0s es anns st = (es', eqs', st') ->
       Forall (wt_exp G (vars++(st_tys st'))) es'.
   Proof.
     intros G vars e0s es anns es' eqs' st st' Hwt1 Hwt2 Hty1 Hty2 Hclock Hnorm.
     unfold normalize_fby in Hnorm. repeat inv_bind.
-    eapply map_bind2_wt_exp' in H; eauto.
-    - destruct a as [[e0 e] a]. eauto.
-    - solve_forall. destruct x as [[e0 e] [ty cl]].
-      unfold fby_iteexp in H1.
-      destruct (Norm.is_constant e0); repeat inv_bind.
-      + repeat rewrite_Forall_forall.
-        repeat constructor; simpl.
-        * repeat simpl_In.
-          apply Hwt1 in H8.
-          repeat solve_incl.
-        * repeat simpl_In.
-          apply Hwt2 in H7.
-          repeat solve_incl.
-        * rewrite app_nil_r.
-          repeat rewrite_Forall_forall.
-          repeat simpl_nth; repeat simpl_length.
-          specialize (H4 _ _ _ _ _ H0 H11 H10). simpl in H4.
-          congruence.
-        * rewrite app_nil_r. repeat simpl_nth; repeat simpl_length.
-          specialize (H6 _ _ _ _ _ H0 H8 H10); simpl in H6.
-          congruence.
-        * repeat simpl_In.
-          apply Hclock in H0. repeat solve_incl.
-      + repeat rewrite_Forall_forall.
-        repeat simpl_length.
-        repeat constructor; simpl.
-        * apply init_var_for_clock_In in H1.
+    eapply map_bind2_wt_exp' in H; eauto; clear H.
+    - destruct a as [[e0 e] a]; eauto.
+    - assert (length e0s = length anns) as Hlen1 by (eapply Forall2_length in Hty1; solve_length).
+      assert (length es = length anns) as Hlen2 by (eapply Forall2_length in Hty2; solve_length).
+      solve_forall. destruct z as (ty, ck).
+      unfold fby_iteexp in H3.
+      destruct (Norm.is_constant x); repeat inv_bind.
+      + repeat constructor; simpl.
+        1,2,5:repeat solve_incl.
+        1,2:rewrite app_nil_r; auto.
+      + inv H6. repeat constructor; simpl.
+        2,3,5,7:repeat solve_incl.
+        * apply init_var_for_clock_In in H3; simpl in H3.
           apply in_or_app; right.
-          eapply fresh_ident_st_follows in H4. eapply st_follows_incl in H4.
-          eapply st_follows_incl in H3.
-          eapply H4 in H1. eapply H3 in H1; simpl in H1.
+          eapply fresh_ident_st_follows, st_follows_incl in H10.
+          eapply st_follows_incl in H5. eapply H10, H5 in H3.
           unfold st_tys, idty. rewrite map_map; simpl.
-          repeat simpl_In. exists (x, (Op.bool_type, (fst cl), true)); auto.
-        * repeat simpl_In. apply Hclock in H0. inv H0. repeat solve_incl.
-        * repeat simpl_In. apply Hwt1 in H10. repeat solve_incl.
-        * apply fresh_ident_In in H4.
-          apply st_follows_tys_incl in H3.
-          apply in_or_app; right. apply H3.
-          rewrite st_anns_tys_In. exists (fst cl). exists false. assumption.
-        * repeat simpl_In. apply Hclock in H0. inv H0. repeat solve_incl.
-        * rewrite app_nil_r.
-          repeat simpl_nth. repeat simpl_length.
-          specialize (H8 _ _ _ _ _ H0 H10 H12). simpl in H8.
-          congruence.
-        * repeat simpl_In. apply Hclock in H0. repeat solve_incl.
+          repeat simpl_In. exists (x1, (Op.bool_type, ck0, true)); auto.
+        * apply fresh_ident_In in H10.
+          apply st_follows_tys_incl in H5.
+          apply in_or_app; right. apply H5.
+          rewrite st_anns_tys_In. exists ck0. exists false. assumption.
+        * rewrite app_nil_r; auto.
   Qed.
 
   Corollary normalize_fby_wt_exp' : forall G vars e0s es anns e0s' es' res eqs1 eqs2 eqs3 st st' st'' st''',
-      wt_exp G vars (Efby e0s es anns) ->
+      wt_exp G (vars++st_tys st) (Efby e0s es anns) ->
       normalize_exps e0s st = (e0s', eqs1, st') ->
       normalize_exps es st' = (es', eqs2, st'') ->
       normalize_fby e0s' es' anns st'' = (res, eqs3, st''') ->
       Forall (wt_exp G (vars++st_tys st''')) res.
   Proof with eauto.
-    intros G vars e0s es anns e0s' es' res eqs1 eqs2 eqs3 st st' st'' st''' Hwc Hnorm1 Hnorm2 Hnorm3.
+    intros * Hwc Hnorm1 Hnorm2 Hnorm3.
     inv Hwc. eapply normalize_fby_wt_exp. 6:eauto.
     - eapply normalize_exps_wt_exp with (G:=G) (vars:=vars) in Hnorm1...
       1,2:solve_forall; repeat solve_incl.
     - eapply normalize_exps_wt_exp with (G:=G) (vars:=vars) in Hnorm2...
-    - clear Hnorm3 Hnorm2 H3 H4.
-      assert (length e0s' = length (annots e0s)) by eauto.
-      specialize (normalize_exps_numstreams _ _ _ _ _ Hnorm1) as Hnumstreams.
-      unfold normalize_exps in Hnorm1; repeat inv_bind.
-      eapply map_bind2_normalize_exp_typesof' in H0...
-      assert (Forall2 eq (map typesof x) (map typeof e0s)).
-      { specialize (Forall2_map_1 (fun tys e => tys = typeof e) typesof x e0s) as [_ Hfm].
-        specialize (Forall2_map_2 (fun tys tys' => tys = tys') typeof (map typesof x) e0s) as [_ Hfm2].
-        auto. } rewrite Forall2_eq in H1.
-      repeat rewrite_Forall_forall.
-      + rewrite <- length_typesof_annots, typesof_annots in *. solve_length.
-      + setoid_rewrite (concat_length_map_nth _ _ _ _ _)...
-        * repeat simpl_list.
-          replace (concat (map typeof (concat x))) with (concat (map typeof e0s)).
-          2: { rewrite <- H1. rewrite typeof_concat_typesof... } clear H1.
-          rewrite H5, map_nth...
-        * solve_forall. rewrite length_typeof_numstreams...
-    - clear Hnorm1 Hnorm3 H2 H5 H6.
-      assert (length es' = length (annots es)) by eauto.
-      specialize (normalize_exps_numstreams _ _ _ _ _ Hnorm2) as Hnumstreams.
-      unfold normalize_exps in Hnorm2; repeat inv_bind.
-      eapply map_bind2_normalize_exp_typesof' in H0...
-      assert (Forall2 (fun tys tys' => tys = tys') (map typesof x) (map typeof es)).
-      { specialize (Forall2_map_1 (fun tys e => tys = typeof e) typesof x es) as [_ Hfm].
-        specialize (Forall2_map_2 (fun tys tys' => tys = tys') typeof (map typesof x) es) as [_ Hfm2].
-        auto. } rewrite Forall2_eq in H1.
-      repeat rewrite_Forall_forall.
-      -- rewrite <- length_typesof_annots in *. solve_length.
-      -- setoid_rewrite (concat_length_map_nth _ _ _ _ _)...
-         ++ repeat simpl_list.
-            replace (concat (map typeof (concat x))) with (concat (map typeof es)).
-            2: { rewrite <- H1. rewrite typeof_concat_typesof... } clear H1.
-            rewrite H4, map_nth...
-         ++ solve_forall. rewrite length_typeof_numstreams...
+      solve_forall; repeat solve_incl.
+    - unfold normalize_exps in Hnorm1; repeat inv_bind.
+      eapply map_bind2_normalize_exp_typesof'' in H... congruence.
+    - unfold normalize_exps in Hnorm2; repeat inv_bind.
+      eapply map_bind2_normalize_exp_typesof'' in H... congruence.
     - rewrite Forall_map in H6.
       eapply Forall_impl; [| eauto]. intros [? ?] ?...
+      repeat solve_incl.
   Qed.
 
   Fact normalize_reset_typeof_bool : forall e e' eqs' st st',
@@ -751,9 +681,9 @@ Fact normalize_fby_wt_exp : forall G vars e0s es anns es' eqs' st st',
   Qed.
 
   Fact normalize_rhs_wt_exp : forall G vars e keep_fby es' eqs' st st',
-      wt_exp G vars e ->
+      wt_exp G (vars++st_tys st) e ->
       normalize_rhs keep_fby e st = (es', eqs', st') ->
-      Forall (wt_exp G (vars++(st_tys st'))) es'.
+      Forall (wt_exp G (vars++st_tys st')) es'.
   Proof with eauto.
     intros G vars e keep_fby es' eqs' st st' Hwt Hnorm.
     destruct e; unfold normalize_rhs in Hnorm;
@@ -770,17 +700,17 @@ Fact normalize_fby_wt_exp : forall G vars e0s es anns es' eqs' st st',
       1,2:replace (fresh_ins x) with (@nil (ident * (Op.type * clock))); simpl. 2,4:(eapply normalize_exps_no_fresh in H; eauto).
       3,4: (eapply normalize_exps_typesof in H; eauto; congruence).
       + unfold idty in *. rewrite <- app_assoc, map_app in *.
-        solve_incl. eapply incl_appr', incl_appl'.
+        solve_incl. eapply incl_appr', incl_app; [apply incl_appl; repeat solve_incl|apply incl_app]; auto.
         apply normalize_exps_fresh_incl in H.
-        unfold st_tys, idty. eapply incl_map...
+        unfold st_tys, idty. apply incl_appl, incl_map...
       + unfold idty in *. rewrite <- app_assoc, map_app in *.
-        solve_incl. eapply incl_appr', incl_appl'.
+        solve_incl. eapply incl_appr', incl_app; [apply incl_appl; repeat solve_incl|apply incl_app]; auto.
         apply normalize_exps_fresh_incl in H.
         assert (st_follows x1 st') by repeat solve_st_follows.
-        unfold st_tys, idty. eapply incl_map.
+        unfold st_tys, idty. eapply incl_appl, incl_map.
         etransitivity... eapply incl_map...
       + specialize (normalize_exp_no_fresh _ _ _ _ _ _ H0) as Hincl.
-        eapply normalize_exp_wt_exp in H0...
+        eapply normalize_exp_wt_exp with (G:=G) (vars:=vars) in H0... 2:repeat solve_incl.
         eapply hd_default_wt_exp in H0.
         eapply normalize_reset_wt_exp in H1...
         destruct x4; simpl; try apply incl_nil'.
@@ -796,16 +726,16 @@ Fact normalize_fby_wt_exp : forall G vars e0s es anns es' eqs' st st',
   Qed.
 
   Corollary normalize_rhss_wt_exp : forall G vars es keep_fby es' eqs' st st',
-      Forall (wt_exp G vars) es ->
+      Forall (wt_exp G (vars++st_tys st)) es ->
       normalize_rhss keep_fby es st = (es', eqs', st') ->
-      Forall (wt_exp G (vars++(st_tys st'))) es'.
+      Forall (wt_exp G (vars++st_tys st')) es'.
   Proof with eauto.
     intros G vars es keep_fby es' eqs' st st' Hwt Hnorm.
     unfold normalize_rhss in Hnorm; repeat inv_bind.
     eapply map_bind2_wt_exp in H...
     solve_forall.
-    eapply normalize_rhs_wt_exp in H1...
-    solve_forall. repeat solve_incl.
+    eapply normalize_rhs_wt_exp with (G:=G) (vars:=vars) in H2...
+    solve_forall. 1,2:repeat solve_incl.
   Qed.
 
   Fact map_bind2_wt_eq {A A1 B} :
@@ -859,13 +789,13 @@ Fact normalize_fby_wt_exp : forall G vars e0s es anns es' eqs' st st',
   Qed.
 
   Fact normalize_fby_wt_eq : forall G vars e0s es anns es' eqs' st st',
-      Forall (wt_exp G (vars++(st_tys st))) e0s ->
-      Forall (wt_exp G (vars++(st_tys st))) es ->
-      Forall2 (fun e0 a => typeof e0 = [fst a]) e0s anns ->
-      Forall2 (fun e a => typeof e = [fst a]) es anns ->
-      Forall (fun '(_, cl) => wt_nclock vars cl) anns ->
+      Forall (wt_exp G (vars++st_tys st)) e0s ->
+      Forall (wt_exp G (vars++st_tys st)) es ->
+      Forall2 (fun e0 a => typeof e0 = [a]) e0s (map fst anns) ->
+      Forall2 (fun e a => typeof e = [a]) es (map fst anns) ->
+      Forall (fun '(_, cl) => wt_nclock (vars++st_tys st) cl) anns ->
       normalize_fby e0s es anns st = (es', eqs', st') ->
-      Forall (wt_equation G (vars++(st_tys st'))) eqs'.
+      Forall (wt_equation G (vars++st_tys st')) eqs'.
   Proof with eauto.
     intros G vars e0s es anns es' eqs' st st' Hwt1 Hwt2 Hty1 Hty2 Hclock Hnorm.
     unfold normalize_fby in Hnorm. repeat inv_bind.
@@ -879,12 +809,13 @@ Fact normalize_fby_wt_exp : forall G vars e0s es anns es' eqs' st st',
           eapply add_whens_wt_exp...
           -- simpl. f_equal... apply Op.type_init_type.
           -- eapply Hclock in H4. destruct cl; simpl. inv H4.
-             solve_incl.
+             repeat solve_incl.
         * repeat simpl_In.
           apply Hwt2 in H8. repeat solve_incl.
         * rewrite app_nil_r.
           repeat simpl_nth. repeat simpl_length.
-          specialize (H1 _ _ _ _ _ H4 H13 H12); simpl in H1. congruence.
+          rewrite split_nth in H12. inv H12. rewrite split_map_fst in *.
+          specialize (H1 _ _ _ _ _ H4 H13 H15); simpl in H1. congruence.
         * rewrite app_nil_r.
           apply add_whens_typeof; simpl.
           f_equal. apply Op.type_init_type.
@@ -945,7 +876,7 @@ Fact normalize_fby_wt_exp : forall G vars e0s es anns es' eqs' st st',
     induction anns; intros ids st st' Hidents Hf;
       repeat inv_bind; simpl; auto.
     inv Hf. destruct a as [ty [cl ?]].
-    destruct o; repeat inv_bind; econstructor.
+    destruct o; repeat inv_bind; simpl; constructor.
     - repeat constructor; simpl.
       inv H1. destruct x; simpl in *. solve_incl.
       eapply incl_appr', incl_tl', incl_app.
@@ -954,7 +885,7 @@ Fact normalize_fby_wt_exp : forall G vars e0s es anns es' eqs' st st',
       + apply incl_appr. solve_incl.
     - eapply IHanns in H0.
       + solve_forall. repeat solve_incl.
-      + solve_forall. destruct a, x. solve_incl.
+      + solve_forall. destruct x. solve_incl.
         rewrite Permutation.Permutation_middle.
         eapply incl_appr', incl_appr', incl_cons; try solve_incl.
         eapply reuse_ident_In in H. unfold st_tys, idty, idty.
@@ -968,13 +899,13 @@ Fact normalize_fby_wt_exp : forall G vars e0s es anns es' eqs' st st',
       + apply incl_appr. solve_incl.
     - eapply IHanns in H0.
       + solve_forall.
-      + solve_forall. destruct a. solve_incl.
+      + solve_forall. solve_incl.
         eapply incl_appr', incl_appr'. solve_incl.
   Qed.
 
   Import Permutation.
   Fact normalize_exp_wt_eq : forall G vars e is_control es' eqs' st st',
-      wt_exp G vars e ->
+      wt_exp G (vars++st_tys st) e ->
       normalize_exp is_control e st = (es', eqs', st') ->
       Forall (wt_equation G (vars++(st_tys st'))) eqs'.
   Proof with eauto.
@@ -986,23 +917,24 @@ Fact normalize_fby_wt_exp : forall G vars e0s es anns es' eqs' st st',
     - (* binop *)
       inv Hwt.
       rewrite Forall_app.
-      split; eauto.
-      eapply IHe1 in H; eauto.
-      solve_forall. eapply wt_equation_incl; [| eauto].
-      eapply normalize_exp_st_follows in H0.
-      repeat solve_incl.
+      split.
+      + eapply IHe1 in H; eauto.
+        solve_forall. eapply wt_equation_incl; [| eauto].
+        eapply normalize_exp_st_follows in H0.
+        repeat solve_incl.
+      + eapply IHe2 in H0; eauto.
+        repeat solve_incl.
     - (* fby *)
       inv Hwt.
       repeat rewrite Forall_app.
-      repeat split; eauto.
+      repeat split.
       + rewrite Forall_map.
-        solve_forall.
-        destruct x as [[x ?] ?].
+        apply Forall_forall. intros [[? ?] ?] ?.
         repeat constructor.
         * repeat simpl_In.
           eapply normalize_fby_wt_exp' with (G:=G) (vars:=vars) in H3.
           3,4: (unfold normalize_exps; inv_bind; repeat eexists; [| inv_bind; eauto]; eauto).
-          2:eauto.
+          2:constructor; eauto.
           rewrite Forall_forall in H3. apply H3 in H5. repeat solve_incl.
         * clear H H0 H12.
           specialize (normalize_fby_numstreams _ _ _ _ _ _ _ H3) as Hnumstreams. rewrite Forall_forall in Hnumstreams.
@@ -1021,7 +953,7 @@ Fact normalize_fby_wt_exp : forall G vars e0s es anns es' eqs' st st',
           apply normalize_fby_typeof in H3; solve_length.
           repeat simpl_nth.
           unfold idty. repeat simpl_In.
-          exists (x, a0); simpl... split.
+          exists (i, a0); simpl... split.
           -- f_equal.
              apply idents_for_anns_values in H4; symmetry in H4. rewrite <- Forall2_eq in H4.
              rewrite Forall2_forall2 in H4; destruct H4 as [_ H4].
@@ -1040,209 +972,120 @@ Fact normalize_fby_wt_exp : forall G vars e0s es anns es' eqs' st st',
              eapply nth_In in H5. setoid_rewrite H14 in H5. assumption.
       + eapply map_bind2_wt_eq in H1; eauto.
         rewrite Forall_forall in *; intros.
-        specialize (H _ H5 _ _ _ _ _ (H8 _ H5) H6).
-        solve_forall. repeat solve_incl.
+        assert (H':=H). eapply H in H6; auto.
+        solve_forall; repeat solve_incl.
+        apply H8 in H5; repeat solve_incl.
       + eapply map_bind2_wt_eq in H2; eauto.
         rewrite Forall_forall in *; intros.
-        specialize (H0 _ H5 _ _ _ _ _ (H9 _ H5) H6).
-        solve_forall. repeat solve_incl.
+        apply H0 in H6; auto.
+        solve_forall; repeat solve_incl.
+        apply H9 in H5; repeat solve_incl.
       + eapply normalize_fby_wt_eq with (G:=G) (vars:=vars) in H3...
         * solve_forall. repeat solve_incl.
         * eapply map_bind2_normalize_exp_wt_exp in H1...
-          solve_forall. repeat solve_incl.
+          solve_forall; repeat solve_incl.
         * eapply map_bind2_normalize_exp_wt_exp in H2...
-        * specialize (map_bind2_normalize_exp_numstreams _ _ _ _ _ _ H1) as Hnumstreams.
-          eapply map_bind2_normalize_exp_typesof in H1...
-          rewrite <- Forall2_map_2 with (P:=(fun e0 a => typeof e0 = [a])) (f:=fst).
-          rewrite <- H11. rewrite <- H1.
-          clear H1 H3 H10. induction x2; simpl in *...
-          rewrite Forall_app in Hnumstreams; destruct Hnumstreams.
-          repeat simpl_list.
-          apply Forall2_app... clear IHx2.
-          induction a0; simpl...
-          inv H1. rewrite <- length_typeof_numstreams in H7. singleton_length.
-          constructor...
-        * specialize (map_bind2_normalize_exp_numstreams _ _ _ _ _ _ H2) as Hnumstreams.
-          eapply map_bind2_normalize_exp_typesof in H2...
-          rewrite <- Forall2_map_2 with (P:=(fun e0 a => typeof e0 = [a])) (f:=fst).
-          rewrite <- H10. rewrite <- H2.
-          clear H2 H3 H11. induction x9; simpl in *...
-          rewrite Forall_app in Hnumstreams; destruct Hnumstreams.
-          repeat simpl_list.
-          apply Forall2_app... clear IHx9.
-          induction a0; simpl...
-          inv H2. rewrite <- length_typeof_numstreams in H7. singleton_length.
-          constructor...
+          solve_forall; repeat solve_incl.
+        * eapply map_bind2_normalize_exp_typesof'' in H1... congruence.
+        * eapply map_bind2_normalize_exp_typesof'' in H2... congruence.
         * rewrite Forall_forall in *; intros [ty cl] Hin.
-          apply H12. repeat simpl_In. exists (ty, cl)...
+          eapply wt_nclock_incl.
+          2: apply H12; repeat simpl_In; exists (ty, cl)...
+          repeat solve_incl.
     - (* when *)
       inv Hwt; repeat inv_bind.
       eapply map_bind2_wt_eq; eauto.
-      rewrite Forall_forall in *; intros.
-      eapply H in H2. 2,3: eauto.
-      solve_forall.
-      eapply wt_equation_incl; [| eauto]. repeat solve_incl.
+      solve_forall. eapply H5 in H2...
+      solve_forall. 1,2:repeat solve_incl.
     - (* merge *)
       inv Hwt.
+      simpl_forall.
       destruct is_control; repeat inv_bind; repeat rewrite Forall_app; repeat split.
       1,4: eapply map_bind2_wt_eq in H1... 3,5: eapply map_bind2_wt_eq in H2...
-      1,2,3,4:repeat rewrite_Forall_forall.
-      Local Ltac mergeiteeqs Hin1 Hin2 Hind Hnorm :=
-        eapply Hind in Hnorm; eauto;
-        rewrite Forall_forall in Hnorm; eapply Hnorm in Hin2;
-        repeat solve_incl.
-      + mergeiteeqs H3 H12 H H4.
-      + mergeiteeqs H4 H13 H H8.
-      + mergeiteeqs H3 H12 H0 H4.
-      + mergeiteeqs H4 H13 H0 H8.
-      + solve_forall.
-        destruct x0 as [xs es].
-        assert (length (concat x3) = length (annots ets)) as Hlen1 by eauto.
-        assert (length (concat x7) = length (annots efs)) as Hlen2 by eauto.
-        specialize (idents_for_anns_length _ _ _ _ H3) as Hlen3.
-        repeat constructor. rewrite <- length_typesof_annots in *.
-        -- specialize (idents_for_anns_st_follows _ _ _ _ H3) as Hfollows.
-           apply idents_for_anns_values in H3; symmetry in H3. rewrite <- Forall2_eq in H3.
-           repeat rewrite_Forall_forall. repeat simpl_length.
-           repeat simpl_nth. repeat simpl_length.
-           destruct (nth x9 _ _) eqn:Hnth1 in H16; subst.
-           destruct (nth x9 _ _) as [[? ?] ?] eqn:Hnth2 in H17; subst.
-           erewrite combine_nth in Hnth2; [| solve_length]; inv Hnth2.
-           erewrite combine_nth in H13; [| solve_length]; inv H13.
-           simpl in H11. destruct x1; [clear H11| omega]. simpl in H12; subst.
-           constructor; simpl.
-           ++ rewrite <- H16; repeat constructor.
-              eapply map_bind2_normalize_exp_wt_exp in H1; solve_forall.
-              rewrite Forall_forall in H1.
-              rewrite <- Hlen1 in l. eapply nth_In in l. apply H1 in l.
-              eapply wt_exp_incl; [| eauto]. repeat solve_incl.
-           ++ rewrite <- H17; repeat constructor.
-              eapply map_bind2_normalize_exp_wt_exp in H2; solve_forall.
-              rewrite Forall_forall in H2.
-              rewrite <- Hlen2 in l2. eapply nth_In in l2. apply H2 in l2.
-              eapply wt_exp_incl; [| eauto]. repeat solve_incl.
-           ++ eapply nth_In in H7. rewrite H14 in H7.
-              apply in_or_app...
-           ++ rewrite app_nil_r.
-              specialize (map_bind2_normalize_exp_numstreams _ _ _ _ _ _ H1) as Hnumstreams.
-              eapply map_bind2_normalize_exp_typesof in H1; [| rewrite Forall_forall in *; intros; auto].
-              rewrite <- H16. rewrite <- H15. rewrite <- typesof_annots. rewrite <- H1.
-              erewrite concat_length_map_nth.
-              repeat simpl_list...
-              solve_length.
-              solve_forall. rewrite length_typeof_numstreams...
-           ++ rewrite app_nil_r.
-              specialize (map_bind2_normalize_exp_numstreams _ _ _ _ _ _ H2) as Hnumstreams.
-              eapply map_bind2_normalize_exp_typesof in H2; [| rewrite Forall_forall in *; intros; auto].
-              rewrite <- H15. rewrite <- H17. repeat rewrite <- typesof_annots in *. replace (typesof efs) in *. rewrite <- H2.
-              erewrite concat_length_map_nth.
-              repeat simpl_list...
-              solve_length.
-              solve_forall. rewrite length_typeof_numstreams...
-           ++ repeat solve_incl.
-              Unshelve. 1,3,4: exact (hd_default []). exact Op.bool_type. exact (x, default_ann).
-        -- rewrite <- length_typesof_annots in *.
-           repeat simpl_nth. repeat simpl_length.
-           Unshelve. 2,5: exact (hd_default []). 3,4:exact (xH, default_ann). 2,3:exact (hd_default [], hd_default [], Op.bool_type).
-           destruct (nth x0 x6 _) eqn:Hnth1.
-           destruct (nth x0 (combine _ _) _) as [[? ?] ?] eqn:Hnth2.
-           simpl. repeat constructor; subst.
-           repeat simpl_nth. Unshelve. 2:exact default_ann.
-           apply in_or_app. right. apply (idents_for_anns_incl_ty _ _ _ _ H3).
-           apply idents_for_anns_values in H3; symmetry in H3; rewrite <- Forall2_eq in H3.
-           rewrite Forall2_map_1, Forall2_map_1, Forall2_map_2 in H3.
-           rewrite Forall2_forall2 in H3; destruct H3 as [_ H3].
-           specialize (H3 default_ann (xH, default_ann) _ _ _ H4 eq_refl eq_refl).
-           rewrite Hnth1 in H3; simpl in H3.
-           destruct a as [? [? ?]]. inversion H3; rewrite H14.
-           unfold idty. repeat simpl_In.
-           exists (i, (t, (c, o))); subst; split; simpl; auto.
-           setoid_rewrite <- Hnth1.
-           eapply nth_In; solve_length.
+      1,2,3,4:(eapply Forall_impl; eauto;
+               intros ? [Hwt Hf] ? ? ? ? Hnorm ? ?; simpl in *; eapply Hf in Hnorm; [solve_forall|]; repeat solve_incl).
+      simpl_forall.
+      remember (normalize_merge x (concat x3) (concat x7) (typesof ets) nck) as merges.
+      assert (Forall (wt_exp G (vars++st_tys st')) merges).
+      { subst. apply normalize_merge_wt_exp; auto.
+        - assert (incl (vars ++ st_tys st) (vars ++ st_tys st')) by repeat solve_incl; eauto.
+        - repeat solve_incl.
+        - eapply map_bind2_normalize_exp_wt_exp with (G:=G) (vars:=vars) in H1...
+          1,2:solve_forall; repeat solve_incl.
+        - eapply map_bind2_normalize_exp_wt_exp with (G:=G) (vars:=vars) in H2...
+          1,2:solve_forall; repeat solve_incl.
+        - eapply map_bind2_normalize_exp_typesof'' in H1...
+          solve_forall.
+        - eapply map_bind2_normalize_exp_typesof'' in H2... congruence.
+          solve_forall.
+      }
+      assert (length (concat x3) = length (typesof ets)) as Hlen1.
+      { eapply map_bind2_normalize_exp_length in H1; eauto; solve_length. solve_forall. }
+      assert (length (concat x7) = length (typesof efs)) as Hlen2.
+      { clear H9. eapply map_bind2_normalize_exp_length in H2; eauto; solve_length. solve_forall. }
+      assert (Forall2 (fun '(ty, _) e => annot e = [(ty, nck)]) (map snd x6) merges) as Htys.
+      { eapply idents_for_anns_values in H3. rewrite H3, Forall2_map_1.
+        subst; eapply normalize_merge_annot; eauto. congruence. } rewrite Forall2_map_1 in Htys.
+      eapply Forall2_ignore1' with (xs:=x6) in H4.
+      2:{ subst. apply idents_for_anns_length in H3. rewrite map_length in H3.
+          rewrite normalize_merge_length... congruence. }
+      solve_forall.
+      repeat constructor... destruct a; simpl in *.
+      rewrite typeof_annot, H6, app_nil_r; simpl.
+      constructor; auto.
+      assert (In (i, t) (idty x6)).
+      { unfold idty. rewrite in_map_iff. exists (i, (t, n)); eauto. }
+      eapply idents_for_anns_incl_ty in H3.
+      eapply in_or_app, or_intror...
     - (* ite *)
       inv Hwt.
+      eapply Forall_Forall in H; eauto.
+      eapply Forall_Forall in H0; eauto.
       destruct is_control; repeat inv_bind; repeat rewrite Forall_app; repeat split.
-      1,5: eapply IHe in H1; eauto; solve_forall; repeat solve_incl.
+      1,5:eapply IHe in H1; eauto; solve_forall; repeat solve_incl...
       1,4: eapply map_bind2_wt_eq in H2... 3,5: eapply map_bind2_wt_eq in H3...
-      1,2,3,4:repeat rewrite_Forall_forall.
-      + mergeiteeqs H4 H14 H H9.
-      + mergeiteeqs H9 H15 H H12.
-      + mergeiteeqs H4 H14 H0 H9.
-      + mergeiteeqs H9 H15 H0 H12.
-      + solve_forall.
-        destruct x2 as [xs es].
-        assert (length (concat x5) = length (annots ets)) as Hlen1 by eauto.
-        assert (length (concat x9) = length (annots efs)) as Hlen2 by eauto.
-        specialize (idents_for_anns_length _ _ _ _ H4) as Hlen3.
-        repeat constructor. rewrite <- length_typesof_annots in *.
-        -- specialize (idents_for_anns_st_follows _ _ _ _ H4) as Hfollows.
-           apply idents_for_anns_values in H4; symmetry in H4; rewrite <- Forall2_eq in H4.
-           repeat rewrite_Forall_forall. repeat simpl_length.
-           repeat simpl_nth. repeat simpl_length.
-           destruct (nth _ _ _) eqn:Hnth1 in H17; subst.
-           destruct (nth _ _ _) as [[? ?] ?] eqn:Hnth2 in H18; subst.
-           erewrite combine_nth in Hnth2; [| solve_length]; inv Hnth2.
-           erewrite combine_nth in H15; [| solve_length]; inv H15.
-           simpl in H13. destruct x3; [clear H13| omega]. simpl in H14; subst.
-           constructor; simpl.
-           ++ apply hd_default_wt_exp.
-              eapply normalize_exp_wt_exp in H1...
-              solve_forall. repeat solve_incl.
-           ++ rewrite <- H17; repeat constructor.
-              eapply map_bind2_normalize_exp_wt_exp in H2; solve_forall.
-              rewrite Forall_forall in H2.
-              rewrite <- Hlen1 in l. eapply nth_In in l. apply H2 in l.
-              eapply wt_exp_incl; [| eauto]. repeat solve_incl.
-           ++ rewrite <- H18; repeat constructor.
-              eapply map_bind2_normalize_exp_wt_exp in H3; solve_forall.
-              rewrite Forall_forall in H3.
-              rewrite <- Hlen2 in l. eapply nth_In in l. apply H3 in l.
-              eapply wt_exp_incl; [| eauto]. repeat solve_incl.
-           ++ assert (length x = numstreams e) as Hlength by eauto.
-              specialize (normalize_exp_numstreams _ _ _ _ _ _ H1) as Hnumstreams.
-              rewrite <- length_typeof_numstreams in Hlength. rewrite H8 in Hlength; simpl in Hlength.
-              eapply normalize_exp_typeof in H1...
-              singleton_length. congruence.
-           ++ rewrite app_nil_r.
-              specialize (map_bind2_normalize_exp_numstreams _ _ _ _ _ _ H2) as Hnumstreams.
-              eapply map_bind2_normalize_exp_typesof in H2; [| rewrite Forall_forall in *; intros; auto].
-              rewrite <- H16. rewrite <- H17. rewrite <- typesof_annots. rewrite <- H2.
-              erewrite concat_length_map_nth.
-              repeat simpl_list...
-              solve_length.
-              solve_forall. rewrite length_typeof_numstreams...
-           ++ rewrite app_nil_r.
-              specialize (map_bind2_normalize_exp_numstreams _ _ _ _ _ _ H3) as Hnumstreams.
-              eapply map_bind2_normalize_exp_typesof in H3; [| rewrite Forall_forall in *; intros; auto].
-              rewrite <- H16. rewrite <- H18. repeat rewrite <- typesof_annots in *; replace (typesof efs) in *. rewrite <- H3.
-              erewrite concat_length_map_nth.
-              repeat simpl_list...
-              solve_length.
-              solve_forall. rewrite length_typeof_numstreams...
-           ++ repeat solve_incl.
-              Unshelve. 1,3,4: exact (hd_default []). exact Op.bool_type. exact (xH, default_ann).
-        -- rewrite <- length_typesof_annots in *.
-           repeat simpl_nth. repeat simpl_length.
-           Unshelve. 2,5: exact (hd_default []). 3,4:exact (xH, default_ann). 2,3:exact (hd_default [], hd_default [], Op.bool_type).
-           destruct (nth x2 x8 _) eqn:Hnth1.
-           destruct (nth x2 (combine _ _) _) as [[? ?] ?] eqn:Hnth2.
-           simpl. repeat constructor; subst.
-           repeat simpl_nth. Unshelve. 2:exact default_ann.
-           apply in_or_app. right. apply (idents_for_anns_incl_ty _ _ _ _ H4).
-           apply idents_for_anns_values in H4; symmetry in H4; rewrite <- Forall2_eq in H4.
-           rewrite Forall2_map_1, Forall2_map_1, Forall2_map_2 in H4.
-           rewrite Forall2_forall2 in H4; destruct H4 as [_ H4].
-           specialize (H4 default_ann (xH, default_ann) _ _ _ H9 eq_refl eq_refl).
-           destruct nck. destruct a as [? [? ?]].
-           rewrite Hnth1 in H4; simpl in H4. inversion H4; rewrite H15.
-           unfold idty. repeat simpl_In.
-           exists (i, (t, (c0, o0))); subst; split...
-           setoid_rewrite <- Hnth1. eapply nth_In; solve_length.
+      1,2,3,4:(eapply Forall_impl; eauto;
+               intros ? [Hwt Hf] ? ? ? ? Hnorm ? ?; simpl in *; eapply Hf in Hnorm; [solve_forall|]; repeat solve_incl).
+      clear IHe.
+      assert (length x = 1) as Hlen.
+      { eapply normalize_exp_length in H1...
+        rewrite H1, <- length_typeof_numstreams, H8; auto. } singleton_length.
+      apply Forall2_combine', Forall2_map_1, Forall2_map_2.
+      remember (normalize_ite e0 (concat x5) (concat x9) (typesof ets) nck) as ites.
+      assert (Forall (wt_exp G (vars++st_tys st')) ites).
+      { subst. apply normalize_ite_wt_exp; auto.
+        - repeat solve_incl.
+        - eapply normalize_exp_wt_exp in H1... inv H1. repeat solve_incl.
+        - eapply normalize_exp_typeof in H1... simpl in H1; rewrite app_nil_r in H1; congruence.
+        - eapply map_bind2_normalize_exp_wt_exp with (G:=G) (vars:=vars) in H2...
+          1,2:solve_forall; repeat solve_incl.
+        - eapply map_bind2_normalize_exp_wt_exp with (G:=G) (vars:=vars) in H3...
+          1,2:solve_forall; repeat solve_incl.
+        - eapply map_bind2_normalize_exp_typesof'' in H2...
+        - eapply map_bind2_normalize_exp_typesof'' in H3... congruence.
+      }
+      assert (length (concat x5) = length (typesof ets)) as Hlen1.
+      { eapply map_bind2_normalize_exp_length in H2; eauto; solve_length. }
+      assert (length (concat x9) = length (typesof efs)) as Hlen2.
+      { clear H10. eapply map_bind2_normalize_exp_length in H3; eauto; solve_length. }
+      assert (Forall2 (fun '(ty, _) e => annot e = [(ty, nck)]) (map snd x8) ites) as Htys.
+      { eapply idents_for_anns_values in H4. rewrite H4, Forall2_map_1.
+        subst; eapply normalize_ite_annot; eauto. congruence. } rewrite Forall2_map_1 in Htys.
+      eapply Forall2_ignore1' with (xs:=x8) in H9.
+      2:{ subst. apply idents_for_anns_length in H4. rewrite map_length in H4.
+          rewrite normalize_ite_length... congruence. }
+      solve_forall.
+      repeat constructor...
+      destruct a; simpl in *.
+      rewrite typeof_annot, app_nil_r, H9; simpl.
+      constructor; auto.
+      assert (In (i, t) (idty x8)).
+      { unfold idty. rewrite in_map_iff. exists (i, (t, n)); eauto. }
+      eapply idents_for_anns_incl_ty in H4.
+      eapply in_or_app, or_intror...
     - (* app *)
       inv Hwt; repeat inv_bind; repeat econstructor; simpl; eauto.
-      1,7: (eapply map_bind2_wt_exp with (vars0:=(vars++(st_tys st'))) in H1; eauto;
-            solve_forall;
-            try eapply normalize_exp_wt_exp in H4; try eapply normalize_exp_wt_exp in H6; eauto;
+      1,7: (eapply map_bind2_normalize_exp_wt_exp in H1; eauto;
             solve_forall; repeat solve_incl).
       1,6: (eapply map_bind2_normalize_exp_typesof in H1; eauto; congruence).
       3,4,9: rewrite app_nil_r.
@@ -1254,12 +1097,13 @@ Fact normalize_fby_wt_exp : forall G vars e0s es anns es' eqs' st st',
           rewrite <- app_assoc. apply incl_appr'.
           rewrite Permutation_app_comm. apply incl_appr'.
           unfold idty. rewrite map_app. apply incl_appr, incl_refl.
-        * solve_forall. destruct a0; simpl in *.
-          solve_incl. apply incl_appr'.
-          unfold idty. rewrite map_app, Permutation_app_comm. apply incl_appr'.
+        * solve_forall.
+          solve_incl. rewrite <- app_assoc. apply incl_appr'.
+          unfold idty. rewrite map_app.
+          apply incl_app; [repeat solve_incl|].
+          apply incl_app; [apply incl_appr|apply incl_appl; auto].
           apply map_bind2_normalize_exp_fresh_incl in H1. eapply incl_map in H1; eauto.
-      + rewrite Forall2_map_1, Forall2_map_2, Forall2_map_2.
-        eapply Forall2_same.
+      + simpl_forall.
         eapply idents_for_anns'_incl_ty in H3.
         eapply Forall_forall; intros [id [ty [cl name]]] Hin; simpl.
         apply in_or_app; right. apply H3.
@@ -1267,9 +1111,8 @@ Fact normalize_fby_wt_exp : forall G vars e0s es anns es' eqs' st st',
       + eapply map_bind2_wt_eq in H1...
         rewrite Forall_forall in *; intros.
         eapply H0 in H4...
-        solve_forall. repeat solve_incl.
-      + rewrite Forall2_map_1, Forall2_map_2, Forall2_map_2.
-        eapply Forall2_same.
+        solve_forall; repeat solve_incl. apply H8 in H2; repeat solve_incl.
+      + simpl_forall.
         eapply idents_for_anns'_incl_ty in H3.
         eapply Forall_forall; intros [id [ty [cl name]]] Hin; simpl.
         apply in_or_app; right. apply H3.
@@ -1282,16 +1125,17 @@ Fact normalize_fby_wt_exp : forall G vars e0s es anns es' eqs' st st',
           rewrite <- app_assoc. apply incl_appr'.
           rewrite Permutation_app_comm. apply incl_appr'.
           unfold idty. rewrite map_app. apply incl_appr, incl_refl.
-        * solve_forall. destruct a0; simpl in *.
-          solve_incl. apply incl_appr'.
-          unfold idty. rewrite map_app, Permutation_app_comm. apply incl_appr'.
+        * solve_forall; simpl in *.
+          solve_incl. rewrite <- app_assoc. apply incl_appr'.
+          unfold idty. rewrite map_app. apply incl_app; [repeat solve_incl|].
+          apply incl_app; [apply incl_appr|apply incl_appl]...
           apply map_bind2_normalize_exp_fresh_incl in H1.
-          assert (st_follows x1 x8) by eauto. apply st_follows_incl in H6. eapply incl_map in H6.
-          assert (st_follows x8 x4) by eauto. apply st_follows_incl in H7. eapply incl_map in H7.
+          assert (st_follows x1 x8) by eauto. eapply st_follows_incl, incl_map in H7.
+          assert (st_follows x8 x4) by eauto. eapply st_follows_incl, incl_map in H8.
           assert (incl (fresh_ins es) (idty (st_anns x4))) by (repeat (etransitivity; eauto)).
           eapply incl_map...
       + specialize (normalize_exp_no_fresh _ _ _ _ _ _ H2) as Hnofresh.
-        eapply normalize_exp_wt_exp in H2...
+        eapply normalize_exp_wt_exp with (G:=G) (vars:=vars) in H2... 2:repeat solve_incl.
         eapply hd_default_wt_exp in H2...
         eapply normalize_reset_wt_exp in H4...
         2:{ destruct x; simpl. apply incl_nil'.
@@ -1310,15 +1154,16 @@ Fact normalize_fby_wt_exp : forall G vars e0s es anns es' eqs' st st',
         * eapply map_bind2_wt_eq in H1; eauto.
           rewrite Forall_forall in *; intros.
           eapply H0 in H6...
-          solve_forall. repeat solve_incl.
+          solve_forall; repeat solve_incl. eapply H8 in H5; repeat solve_incl.
         * eapply H in H2...
           apply normalize_reset_st_follows in H4.
           apply idents_for_anns'_st_follows in H3.
-          solve_forall. repeat solve_incl.
+          solve_forall. 1,2:repeat solve_incl.
         * assert (length x = numstreams r) as Hlength by eauto.
           specialize (normalize_exp_typeof _ _ _ _ _ _ _ _ H13 H2) as Htypeof.
           rewrite H14 in Htypeof.
-          eapply normalize_exp_wt_exp in H2... eapply hd_default_wt_exp in H2...
+          eapply normalize_exp_wt_exp with (G:=G) (vars:=vars) in H2... 2:repeat solve_incl.
+          eapply hd_default_wt_exp in H2...
           eapply normalize_reset_wt_eq in H4...
           -- solve_forall. repeat solve_incl.
           -- rewrite <- length_typeof_numstreams in Hlength. rewrite H14 in Hlength; simpl in Hlength.
@@ -1326,7 +1171,7 @@ Fact normalize_fby_wt_exp : forall G vars e0s es anns es' eqs' st st',
   Qed.
 
   Corollary normalize_exps_wt_eq : forall G vars es es' eqs' st st',
-      Forall (wt_exp G vars) es ->
+      Forall (wt_exp G (vars++st_tys st)) es ->
       normalize_exps es st = (es', eqs', st') ->
       Forall (wt_equation G (vars++(st_tys st'))) eqs'.
   Proof with eauto.
@@ -1334,12 +1179,12 @@ Fact normalize_fby_wt_exp : forall G vars e0s es anns es' eqs' st st',
     unfold normalize_exps in Hnorm. repeat inv_bind.
     eapply map_bind2_wt_eq in H...
     solve_forall.
-    eapply normalize_exp_wt_eq in H1...
-    solve_forall. repeat solve_incl.
+    eapply normalize_exp_wt_eq with (G:=G) (vars:=vars) in H2...
+    solve_forall. 1,2:repeat solve_incl.
   Qed.
 
   Fact normalize_rhs_wt_eq : forall G vars e keep_fby es' eqs' st st',
-      wt_exp G vars e ->
+      wt_exp G (vars++st_tys st) e ->
       normalize_rhs keep_fby e st = (es', eqs', st') ->
       Forall (wt_equation G (vars++(st_tys st'))) eqs'.
   Proof with eauto.
@@ -1352,29 +1197,27 @@ Fact normalize_fby_wt_exp : forall G vars e0s es anns es' eqs' st st',
       repeat rewrite Forall_app. repeat split.
       + eapply normalize_exps_wt_eq in H...
         solve_forall. repeat solve_incl.
-      + eapply normalize_exps_wt_eq in H0...
-        solve_forall. repeat solve_incl.
+      + eapply normalize_exps_wt_eq with (G:=G) (vars:=vars) in H0...
+        1,2:solve_forall; repeat solve_incl.
       + eapply normalize_fby_wt_eq in H1...
         * eapply normalize_exps_wt_exp in H...
           solve_forall. repeat solve_incl.
         * eapply normalize_exps_wt_exp in H0...
+          solve_forall; repeat solve_incl.
         * specialize (normalize_exps_numstreams _ _ _ _ _ H) as Hnumstreams.
           eapply normalize_exps_typesof in H...
-          rewrite <- Forall2_map_2 with (P:=(fun e0 a => typeof e0 = [a])) (f:=fst).
           rewrite <- H5. rewrite <- H.
           clear H H1 H4 H5. induction x; simpl...
           inv Hnumstreams. rewrite <- length_typeof_numstreams in H4. singleton_length.
           constructor...
         * specialize (normalize_exps_numstreams _ _ _ _ _ H0) as Hnumstreams.
           eapply normalize_exps_typesof in H0...
-          rewrite <- Forall2_map_2 with (P:=(fun e0 a => typeof e0 = [a])) (f:=fst).
-          rewrite <- H4. rewrite <- H0.
+          rewrite <- H4, <- H0.
           clear H H0 H1 H4 H5. induction x2; simpl...
           inv Hnumstreams. rewrite <- length_typeof_numstreams in H1. singleton_length.
           constructor...
         * rewrite Forall_forall in *; intros.
-          destruct x5. eapply H6. simpl_In.
-          exists (t, n)...
+          destruct x5. eapply wt_nclock_incl; [|eapply H6; simpl_In; exists (t, n); eauto]; repeat solve_incl.
     - eapply normalize_exp_wt_eq...
     - (* app *)
       repeat inv_bind.
@@ -1383,11 +1226,12 @@ Fact normalize_fby_wt_exp : forall G vars e0s es anns es' eqs' st st',
         solve_forall. repeat solve_incl.
       + inv Hwt; repeat inv_bind; try constructor.
         apply Forall_app. split.
-        * eapply normalize_exp_wt_eq in H0...
-          solve_forall. repeat solve_incl.
+        * eapply normalize_exp_wt_eq with (G:=G) (vars:=vars) in H0...
+          solve_forall. 1,2:repeat solve_incl.
         * eapply normalize_reset_wt_eq with (G:=G) (vars:=vars) in H1...
           -- eapply hd_default_wt_exp.
              eapply normalize_exp_wt_exp in H0...
+             repeat solve_incl.
           -- specialize (normalize_exp_numstreams _ _ _ _ _ _ H0) as Hnumstreams.
              eapply normalize_exp_typeof in H0...
              rewrite H11 in H0.
@@ -1396,27 +1240,28 @@ Fact normalize_fby_wt_exp : forall G vars e0s es anns es' eqs' st st',
   Qed.
 
   Corollary normalize_rhss_wt_eq : forall G vars es keep_fby es' eqs' st st',
-      Forall (wt_exp G vars) es ->
+      Forall (wt_exp G (vars++st_tys st)) es ->
       normalize_rhss keep_fby es st = (es', eqs', st') ->
       Forall (wt_equation G (vars++(st_tys st'))) eqs'.
   Proof with eauto.
     intros G vars es keep_fby es' eqs' st st' Hwt Hnorm.
     unfold normalize_rhss in Hnorm; repeat inv_bind.
     eapply map_bind2_wt_eq in H...
-    solve_forall. eapply normalize_rhs_wt_eq in H1...
-    solve_forall. repeat solve_incl.
+    solve_forall. eapply normalize_rhs_wt_eq with (G:=G) (vars:=vars) in H2...
+    solve_forall. 1,2:repeat solve_incl.
   Qed.
 
   Fact normalize_equation_wt_eq : forall G vars eq to_cut eqs' st st',
-      wt_equation G vars eq ->
+      wt_equation G (vars++st_tys st) eq ->
       normalize_equation to_cut eq st = (eqs', st') ->
-      Forall (wt_equation G (vars++(st_tys st'))) eqs'.
+      Forall (wt_equation G (vars++st_tys st')) eqs'.
   Proof with eauto.
     intros G vars eq to_cut eqs' st st' Hwt Hnorm.
     destruct eq as [xs es]; simpl in Hnorm.
     repeat inv_bind. destruct Hwt.
     apply Forall_app. split.
     - specialize (normalize_rhss_typesof _ _ _ _ _ _ _ _ H0 H) as Htypeof.
+      assert (st_follows st st') as Hfollows by eauto.
       eapply normalize_rhss_wt_exp in H...
       rewrite <- Htypeof in H1.
       clear Htypeof. revert xs H1.
@@ -1433,7 +1278,8 @@ Fact normalize_fby_wt_exp : forall G vars e0s es anns es' eqs' st st',
           specialize (H1 a0 b _ _ _ Hlen2 eq_refl eq_refl).
           rewrite app_nth1 in H1. 2: rewrite length_typeof_numstreams.
           rewrite nth_firstn_1. 2,3:eauto.
-          apply in_or_app...
+          rewrite in_app_iff in *. destruct H1; auto.
+          right. eapply st_follows_tys_incl...
       + inv H. apply IHx...
         repeat rewrite_Forall_forall.
         * rewrite app_length in H.
@@ -1450,16 +1296,17 @@ Fact normalize_fby_wt_exp : forall G vars e0s es anns es' eqs' st st',
   Qed.
 
   Corollary normalize_equations_wt_eq : forall G vars eqs to_cut eqs' st st',
-      Forall (wt_equation G vars) eqs ->
+      Forall (wt_equation G (vars++st_tys st)) eqs ->
       normalize_equations to_cut eqs st = (eqs', st') ->
-      Forall (wt_equation G (vars++(st_tys st'))) eqs'.
+      Forall (wt_equation G (vars++st_tys st')) eqs'.
   Proof with eauto.
     induction eqs; intros to_cut eqs' st st' Hwt Hnorm;
-      repeat inv_bind.
-    - constructor.
-    - inv Hwt. apply Forall_app. split...
-      eapply normalize_equation_wt_eq in H...
-      solve_forall. repeat solve_incl.
+      repeat inv_bind; auto.
+    inv Hwt. apply Forall_app. split.
+    - eapply normalize_equation_wt_eq in H...
+      solve_forall; repeat solve_incl.
+    - eapply IHeqs in H0...
+      solve_forall; repeat solve_incl.
   Qed.
 
   (** ** Preservation of wt_clock *)
@@ -1546,13 +1393,13 @@ Fact normalize_fby_wt_exp : forall G vars e0s es anns es' eqs' st st',
     - eapply map_bind2_st_follows...
       solve_forall...
     - solve_forall.
-      eapply H1 in H2...
+      eapply H2 in H5...
       etransitivity...
   Qed.
 
   Fact normalize_fby_wt_clock : forall vars e0s es anns es' eqs' st st',
       Forall (wt_clock (vars++st_tys st)) (st_clocks st) ->
-      Forall (wt_nclock vars) (map snd anns) ->
+      Forall (wt_nclock (vars++st_tys st)) (map snd anns) ->
       normalize_fby e0s es anns st = (es', eqs', st') ->
       Forall (wt_clock (vars++st_tys st')) (st_clocks st').
   Proof with eauto.
@@ -1560,15 +1407,15 @@ Fact normalize_fby_wt_exp : forall G vars e0s es anns es' eqs' st st',
     unfold normalize_fby in Hnorm. repeat inv_bind.
     eapply map_bind2_wt_clock in H...
     1: intros ? ? [[? ?] ?] ? ? Hfby; eapply fby_iteexp_st_follows...
-    solve_forall. destruct x as [[e0 e] [ty cl]].
+    eapply Forall_forall; intros [[? ?] [? ?]] ? * ? ? ? ?.
     unfold fby_iteexp in H2.
-    destruct (Norm.is_constant e0); repeat inv_bind.
+    destruct (Norm.is_constant e); repeat inv_bind.
     - assumption.
     - repeat simpl_In.
       unfold init_var_for_clock in H2.
-      assert (wt_nclock vars cl) as Hcl.
+      assert (wt_nclock (vars++st_tys st) n) as Hcl.
       { rewrite Forall_forall in Hwt. eapply Hwt.
-        repeat simpl_In. exists (ty, cl)... }
+        repeat simpl_In. exists (t, n)... }
       destruct (find _ _).
       + destruct p. inv H2.
         inv Hcl.
@@ -1603,71 +1450,85 @@ Fact normalize_fby_wt_exp : forall G vars e0s es anns es' eqs' st st',
   Qed.
 
   Fact normalize_exp_wt_clock : forall G vars e is_control es' eqs' st st',
-      wt_exp G vars e ->
+      wt_exp G (vars++st_tys st) e ->
       Forall (wt_clock (vars++st_tys st)) (st_clocks st) ->
       normalize_exp is_control e st = (es', eqs', st') ->
       Forall (wt_clock (vars++st_tys st')) (st_clocks st').
   Proof with eauto.
     induction e using exp_ind2; intros is_control es' eqs' st st' Hwt Hclocks Hnorm;
       inv Hwt; repeat inv_bind; eauto.
+    Ltac solve_map_bind2:=
+      eapply Forall_impl; eauto;
+      intros ? [? Hf] ? ? ? ? ? Hnorm ? ?; eapply Hf in Hnorm; eauto; repeat solve_incl.
+    - (* binop *)
+      eapply IHe2 in H0...
+      repeat solve_incl.
     - (* fby *)
-      eapply map_bind2_wt_clock in H1...
-      2: rewrite Forall_forall in *; intros...
+      eapply idents_for_anns_wt_clock in H9... 2:solve_forall; repeat solve_incl.
+      eapply normalize_fby_wt_clock with (vars:=vars) in H3...
+      1,3:solve_forall; solve_incl; repeat solve_incl.
+      eapply Forall_Forall in H; eauto. clear H4.
+      eapply Forall_Forall in H0; eauto. clear H5.
       eapply map_bind2_wt_clock in H2...
-      2: rewrite Forall_forall in *; intros...
-      eapply normalize_fby_wt_clock in H3...
-      eapply idents_for_anns_wt_clock in H9...
-      1,2: solve_forall; repeat solve_incl.
+      eapply map_bind2_wt_clock in H1...
+      1,2:solve_map_bind2.
     - (* when *)
       eapply map_bind2_wt_clock in H0...
       rewrite Forall_forall in *; intros...
+      eapply H in H3... eapply H4 in H1... repeat solve_incl.
     - (* merge *)
+      eapply Forall_Forall in H; eauto. clear H5. eapply Forall_Forall in H0; eauto. clear H6.
       destruct is_control; repeat inv_bind.
-      1,2: (eapply map_bind2_wt_clock in H1; eauto; [|rewrite Forall_forall in *; intros; eauto];
-            eapply map_bind2_wt_clock in H2; eauto; try (solve [rewrite Forall_forall in *; intros; eauto])).
-      eapply idents_for_anns_wt_clock in H3...
-      1:solve_forall; repeat solve_incl.
-      rewrite map_map; simpl.
-      solve_forall. simpl_In. solve_incl.
+      + eapply map_bind2_wt_clock in H2... 2:solve_map_bind2.
+        eapply map_bind2_wt_clock in H1... solve_map_bind2.
+      + eapply idents_for_anns_wt_clock in H3...
+        2:{ rewrite map_map; simpl. solve_forall. repeat solve_incl. }
+        eapply map_bind2_wt_clock with (vars0:=vars) in H2... 3:solve_map_bind2. solve_forall; repeat solve_incl.
+        eapply map_bind2_wt_clock in H1... solve_map_bind2.
     - (* ite *)
+      eapply Forall_Forall in H; eauto. clear H6. eapply Forall_Forall in H0; eauto. clear H7.
       destruct is_control; repeat inv_bind.
-      1,2: (eapply IHe in H1; eauto;
-            eapply map_bind2_wt_clock in H2; eauto; [|rewrite Forall_forall in *; intros; eauto];
-            eapply map_bind2_wt_clock in H3; eauto; try (solve [rewrite Forall_forall in *; intros; eauto])).
-      eapply idents_for_anns_wt_clock in H4...
-      1: solve_forall; repeat solve_incl.
-      rewrite map_map; simpl.
-      solve_forall. simpl_In. solve_incl.
+      + eapply map_bind2_wt_clock in H3... 2:solve_map_bind2.
+        eapply map_bind2_wt_clock in H2... solve_map_bind2.
+      + eapply idents_for_anns_wt_clock in H4...
+        2:{ rewrite map_map; simpl. solve_forall. repeat solve_incl. }
+        eapply map_bind2_wt_clock with (vars0:=vars) in H3... 3:solve_map_bind2. solve_forall; repeat solve_incl.
+        eapply map_bind2_wt_clock in H2... solve_map_bind2.
     - (* app *)
+      eapply Forall_Forall in H0; eauto; clear H5.
+      assert (st_follows st st') as Hfollows by repeat solve_st_follows.
       assert (incl (fresh_ins es) (idty (st_anns x4))) as Hincl by (apply map_bind2_normalize_exp_fresh_incl in H1; auto).
-      eapply map_bind2_wt_clock in H1...
-      2: rewrite Forall_forall in *; intros...
+      eapply map_bind2_wt_clock in H1... 2:solve_map_bind2.
       eapply idents_for_anns'_wt_clock in H2...
       1: solve_forall; repeat solve_incl.
-      rewrite Forall_map. solve_forall. solve_incl.
-      apply incl_appr'. unfold idty; rewrite map_app; apply incl_app; apply incl_map.
+      rewrite Forall_map. solve_forall; solve_incl.
+      rewrite <- app_assoc. apply incl_appr', incl_app; repeat solve_incl.
+      unfold st_tys, idty; rewrite map_app; apply incl_app; apply incl_map.
       + etransitivity... apply incl_map. solve_incl.
       + apply idents_for_anns'_fresh_incl in H2...
     - (* app (reset) *)
-      assert (st_follows x8 st') by repeat solve_st_follows.
-      assert (st_follows x1 st') by repeat solve_st_follows.
+      eapply Forall_Forall in H0; eauto; clear H5.
+      assert (st_follows st x1) by repeat solve_st_follows. assert (st_follows x1 st') by repeat solve_st_follows.
+      assert (st_follows x1 x8) by eauto. assert (st_follows x8 st') by repeat solve_st_follows.
       assert (incl (fresh_in r) (idty (st_anns x8))) as Hincl1 by (apply normalize_exp_fresh_incl in H2; auto).
       assert (incl (fresh_ins es) (idty (st_anns x1))) as Hincl2 by (apply map_bind2_normalize_exp_fresh_incl in H1; auto).
       assert (length x6 = numstreams r) as Hlength by eauto.
       assert (clocksof x6 = clockof r) as Hannot by eauto.
-      eapply map_bind2_wt_clock in H1...
-      2: { rewrite Forall_forall in *; intros. repeat simpl_In... }
-      eapply H in H2...
+      eapply map_bind2_wt_clock in H1... 2:solve_map_bind2.
+      eapply H in H2... 2:repeat solve_incl.
       eapply normalize_reset_wt_clock in H4...
       2: { apply wt_exp_clockof in H10. rewrite <- Hannot in H10.
            rewrite <- length_typeof_numstreams, H11 in Hlength; simpl in Hlength.
            singleton_length.
            solve_forall. solve_incl.
-           apply incl_appr', incl_map... }
+           rewrite <- app_assoc. apply incl_appr', incl_app...
+           1: apply st_follows_tys_incl; repeat solve_st_follows.
+           unfold st_tys, idty; apply incl_map... }
       eapply idents_for_anns'_wt_clock in H3...
       1: solve_forall; repeat solve_incl.
       rewrite Forall_map. solve_forall. solve_incl.
-      apply incl_appr'. unfold idty; rewrite map_app; apply incl_app; apply incl_map.
+      rewrite <- app_assoc. apply incl_appr', incl_app; repeat solve_incl.
+      unfold st_tys, idty; apply incl_map, incl_app.
       + etransitivity... apply incl_map. solve_incl.
       + apply idents_for_anns'_fresh_incl in H3...
   Qed.
@@ -1683,15 +1544,13 @@ Fact normalize_fby_wt_exp : forall G vars e0s es anns es' eqs' st st',
     eapply map_bind2_wt_clock in H; eauto.
     solve_forall.
     assert (st_follows st0 st0') by eauto.
-    eapply normalize_exp_wt_clock in H2; [|eauto|].
-    - solve_forall. solve_incl.
-      rewrite <- app_assoc. apply incl_appr', incl_app; auto.
-      repeat solve_incl.
-    - solve_forall. solve_incl.
+    eapply normalize_exp_wt_clock with (G:=G) (vars:=vars) in H3; repeat solve_incl.
+    - solve_forall; solve_incl.
+    - solve_forall; solve_incl.
   Qed.
 
   Corollary normalize_rhs_wt_clock : forall G vars e keep_fby es' eqs' st st',
-      wt_exp G vars e ->
+      wt_exp G (vars++st_tys st) e ->
       Forall (wt_clock (vars++st_tys st)) (st_clocks st) ->
       normalize_rhs keep_fby e st = (es', eqs', st') ->
       Forall (wt_clock (vars++st_tys st')) (st_clocks st').
@@ -1702,40 +1561,41 @@ Fact normalize_fby_wt_exp : forall G vars e0s es anns es' eqs' st st',
         inv Hwt; [destruct keep_fby| |].
     - (* fby (keep) *)
       repeat inv_bind.
+      assert (st_follows st x1) by repeat solve_st_follows. assert (st_follows st x4) by repeat solve_st_follows.
       eapply normalize_exps_wt_clock with (G:=G) in H...
       eapply normalize_exps_wt_clock with (G:=G) in H0...
       eapply normalize_fby_wt_clock in H1...
-      1,2:solve_forall; solve_incl.
+      1,2:solve_forall; do 3 solve_incl; apply st_follows_tys_incl; auto.
     - (* fby (don't keep) *) eapply normalize_exp_wt_clock in Hnorm...
     - (* app *)
       repeat inv_bind.
       eapply normalize_exps_wt_clock with (G:=G) in H...
-      solve_forall. solve_incl.
     - (* app (reset) *)
       repeat inv_bind.
       assert (incl (fresh_in r) (idty (st_anns x6))) as Hincl by (eapply normalize_exp_fresh_incl; eauto).
-      assert (st_follows x6 st') as Hfollows by repeat solve_st_follows.
+      assert (st_follows x6 st') as Hfollows2 by repeat solve_st_follows.
       assert (length x4 = numstreams r) as Hlength by eauto.
       assert (clocksof x4 = clockof r) as Hclockof by eauto.
-      specialize (normalize_exp_wt_exp _ _ _ _ _ _ _ _ H8 H0) as Hwt.
+      assert (wt_exp G (vars ++ st_tys x1) r) as Hwt' by repeat solve_incl.
+      assert (st_follows st st') as Hfollows by repeat solve_st_follows.
+      specialize (normalize_exp_wt_exp _ _ _ _ _ _ _ _ Hwt' H0) as Hwt.
       eapply normalize_exps_wt_clock with (G:=G) in H...
       eapply normalize_exp_wt_clock with (G:=G) in H0...
-      eapply normalize_reset_wt_clock in H1...
-      2,3:solve_forall; solve_incl.
-      2:apply incl_appr'; solve_incl.
+      eapply normalize_reset_wt_clock in H1... 2:solve_forall; repeat solve_incl.
       assert (length x4 = 1).
       { rewrite Hlength. rewrite typeof_annot in H9. rewrite <- length_annot_numstreams.
         erewrite <- map_length. rewrite H9. reflexivity. }
       singleton_length.
       rewrite Hclockof.
       eapply wt_exp_clockof in H8.
-      solve_forall. repeat solve_incl.
-      apply incl_map. etransitivity...
-      apply incl_map, st_follows_incl...
+      solve_forall; solve_incl.
+      rewrite <- app_assoc. apply incl_appr'; repeat solve_incl.
+      apply incl_app; repeat solve_incl. unfold st_tys, idty.
+      apply incl_map; etransitivity... apply incl_map. repeat solve_incl.
   Qed.
 
   Corollary normalize_rhss_wt_clock : forall G vars es keep_fby es' eqs' st st',
-      Forall (wt_exp G vars) es ->
+      Forall (wt_exp G (vars++st_tys st)) es ->
       Forall (wt_clock (vars++st_tys st)) (st_clocks st) ->
       normalize_rhss keep_fby es st = (es', eqs', st') ->
       Forall (wt_clock (vars++st_tys st')) (st_clocks st').
@@ -1743,11 +1603,12 @@ Fact normalize_fby_wt_exp : forall G vars e0s es anns es' eqs' st st',
     intros G vars es keep_fby es' eqs' st st' Hwt Hclocks Hnorm.
     unfold normalize_rhss in Hnorm. repeat inv_bind.
     eapply map_bind2_wt_clock in H; eauto.
-    solve_forall. eapply normalize_rhs_wt_clock in H2; eauto.
+    solve_forall. eapply normalize_rhs_wt_clock with (G:=G) in H3; eauto.
+    repeat solve_incl.
   Qed.
 
   Fact normalize_equation_wt_clock : forall G vars eq to_cut eqs' st st',
-      wt_equation G vars eq ->
+      wt_equation G (vars++st_tys st) eq ->
       Forall (wt_clock (vars++st_tys st)) (st_clocks st) ->
       normalize_equation to_cut eq st = (eqs', st') ->
       Forall (wt_clock (vars++st_tys st')) (st_clocks st').
@@ -1759,7 +1620,7 @@ Fact normalize_fby_wt_exp : forall G vars e0s es anns es' eqs' st st',
   Qed.
 
   Corollary normalize_equations_wt_clock : forall G vars eqs to_cut eqs' st st',
-      Forall (wt_equation G vars) eqs ->
+      Forall (wt_equation G (vars++st_tys st)) eqs ->
       Forall (wt_clock (vars++st_tys st)) (st_clocks st) ->
       normalize_equations to_cut eqs st = (eqs', st') ->
       Forall (wt_clock (vars++st_tys st')) (st_clocks st').
@@ -1768,7 +1629,10 @@ Fact normalize_fby_wt_exp : forall G vars e0s es anns es' eqs' st st',
       unfold normalize_equations in Hnorm; repeat inv_bind.
     - assumption.
     - inv Hwt.
+      assert (st_follows st x0) by repeat solve_st_follows.
       eapply normalize_equation_wt_clock in H; eauto.
+      eapply IHeqs in H0; eauto.
+      solve_forall; repeat solve_incl.
   Qed.
 
   Lemma normalize_node_wt : forall G n to_cut Hwl n',
@@ -1781,37 +1645,31 @@ Fact normalize_fby_wt_exp : forall G vars e0s es anns es' eqs' st st',
     repeat constructor; simpl; auto.
     - unfold wt_clocks in *.
       apply Forall_app. split.
-      + solve_forall. destruct a as [_ [_ ck]]. unfold idty in *.
+      + solve_forall. unfold idty in *.
         solve_incl. repeat rewrite map_app. repeat solve_incl.
       + remember (normalize_equations _ _ _) as res.
         destruct res as [eqs st']. symmetry in Heqres.
-        eapply normalize_equations_wt_clock in Heqres; eauto.
+        eapply normalize_equations_wt_clock with (G:=G) in Heqres; eauto.
         * simpl. unfold st_clocks in Heqres.
-          solve_forall. rewrite Forall_forall in Heqres.
-          destruct x as [? [? ck]].
-          eapply wt_clock_incl; [| eapply Heqres].
-          -- unfold idty. repeat rewrite map_app.
-             repeat rewrite <- app_assoc; apply incl_appr'.
-             rewrite Permutation_swap; apply incl_appr', incl_appr'.
-             reflexivity.
-          -- unfold idty in H.
-             repeat simpl_In. inv H.
-             exists (i, (t, ck, b)); simpl; split; auto.
-        * unfold st_clocks. rewrite init_st_anns; simpl.
-          constructor.
+          unfold idty. rewrite Forall_map in Heqres; rewrite Forall_map.
+          eapply Forall_impl; eauto.
+          intros [? [[? ?] ?]] ?; simpl.
+          repeat solve_incl.
+          repeat rewrite map_app, app_assoc.
+          eapply incl_appr'. reflexivity.
+        * unfold st_clocks. unfold st_tys. rewrite init_st_anns, app_nil_r.
+          repeat rewrite <- app_assoc. repeat rewrite <- map_app.
+          solve_forall; repeat solve_incl. apply incl_map, incl_appr'. rewrite Permutation_app_comm; auto.
+        * unfold st_clocks. rewrite init_st_anns; simpl; constructor.
     - remember (normalize_equations _ _ _) as res.
       destruct res as [eqs' st']; simpl.
       symmetry in Heqres.
-      eapply normalize_equations_wt_eq in Heqres; eauto.
-      solve_forall. repeat solve_incl. clear Heqres H.
-      unfold st_tys, idty in *. apply incl_app.
-      + apply incl_map. apply incl_app; [solve_incl|].
-        apply incl_app; [| repeat solve_incl].
-        apply incl_appr. apply incl_appl; solve_incl.
-      + repeat rewrite map_map; simpl.
-        repeat rewrite map_app; simpl.
-        apply incl_appr. apply incl_appl. apply incl_appr.
-        repeat rewrite map_map; simpl. reflexivity.
+      eapply normalize_equations_wt_eq with (G:=G) (vars:=(idty (n_in n ++ n_vars n ++ n_out n))) in Heqres; eauto.
+      + solve_forall; solve_incl.
+        unfold st_tys; rewrite <- idty_app. apply incl_map.
+        repeat rewrite <- app_assoc. apply incl_appr', incl_appr'.
+        rewrite Permutation_app_comm. reflexivity.
+      + solve_forall; repeat solve_incl.
   Qed.
 
   Lemma normalize_global_wt : forall G Hwl G',
